pulse/share/pulse/examples/dice/dpe/DPE.fst
@@ -48,430 +48,6 @@ open Pulse.Lib.Mutex
 assume
 val run_stt (#a:Type) (#post:a -> vprop) (f:stt a emp post) : a
 
-//
-// Concrete state setup
-//
-
-type ctxt_hndl_t = U32.t
-
-type sid_t : eqtype = U32.t
-
-//
-// A session may be in one of the following states
-//
-// InUse is never returned to the client
-//
-[@@ Rust_derive "Clone"]
-noeq
-type session_state =
-  | SessionStart
-  | Available { handle:ctxt_hndl_t; context:context_t }
-  | InUse
-  | SessionClosed
-  | SessionError
-
-type ht_t = ht_t sid_t session_state
-
-//
-// DPE state
-// A counter for next sid
-//   and a hashtable mapping sids to session state
-//
-noeq
-type st = { st_ctr:sid_t; st_tbl:ht_t; }
-
-
-//
-// Ghost state set up
-//
-
-//
-// Ghost session state
-//
-// Has a 1-1 correspondence with the concrete session state
-//   except it has an G_UnInitialized
-//
-[@@ erasable]
-noeq
-type g_session_state : Type u#1 =
-  | G_UnInitialized : g_session_state
-  | G_SessionStart : g_session_state
-  | G_Available : repr:context_repr_t -> g_session_state
-  | G_InUse : g_session_state -> g_session_state
-  | G_SessionClosed : g_session_state -> g_session_state
-  | G_SessionError : g_session_state -> g_session_state
-
-//
-// A relation between context reprs that follow each other
-//
-// L0 repr should use the same UDS as the engine repr,
-//   and L1 repr should use the same CDI as the L0 repr
-//
-noextract
-let next_repr (r1 r2:context_repr_t) : prop =
-  match r1, r2 with
-  | Engine_context_repr uds, L0_context_repr l0_repr ->
-    uds == l0_repr.uds
-  | L0_context_repr l0_repr, L1_context_repr l1_repr ->
-    l0_repr.cdi == l1_repr.cdi
-  | _ -> False
-
-//
-// State machine
-//
-noextract
-let rec next (s0 s1:g_session_state) : prop =
-  match s0, s1 with
-  //
-  // UnInitialized may only go to SessionStart
-  // No other incoming/outgoing edges to/from it
-  //
-  | G_UnInitialized, G_SessionStart -> True
-  | G_UnInitialized, _
-  | _, G_UnInitialized -> False
-
-  //
-  // SessionStart may go to Available with engine repr
-  //
-  | G_SessionStart, G_Available (Engine_context_repr _) -> True
-
-  //
-  // Available r0 may go to Available r1,
-  //   as long as repr r1 follows repr r0
-  //
-  | G_Available r0, G_Available r1 -> next_repr r0 r1
-
-  //
-  // SessionClosed is a terminal state
-  //
-  | G_SessionClosed _, _ -> False
-
-  //
-  // From any state we can go to InUse, SessionClosed, or SessionError
-  //
-  // These states capture the previous state
-  //
-  | _, G_InUse s -> s == s0
-  | _, G_SessionClosed s
-  | _, G_SessionError s -> s == s0
-
-  //
-  // From InUse s we can go to s1, as long as s can go to s1
-  //
-  | G_InUse s, s1 -> next s s1
-
-  | _ -> False
-
-
-//
-// Defining traces
-//
-
-noextract
-let rec well_formed_trace (l:list g_session_state) : prop =
-  match l with
-  | []
-  | [G_SessionStart] -> True
-  | s1::s0::tl -> next s0 s1 /\ well_formed_trace (s0::tl)
-  | _ -> False
-
-noextract
-type trace_elt : Type u#1 = l:list g_session_state { well_formed_trace l }
-
-noextract
-let trace_extension (t0 t1:trace_elt) : prop =
-  Cons? t1 /\ t0 == List.Tot.tail t1
-
-noextract
-let trace_preorder : FStar.Preorder.preorder trace_elt =
-  FStar.ReflexiveTransitiveClosure.closure trace_extension
-
-noextract
-type trace = hist trace_preorder
-
-noextract
-type trace_pcm_t : Type u#1 = FP.pcm_carrier trace_preorder
-
-//
-// Trace PCM is fractional preorder PCM,
-//   with trace preorder
-//
-noextract
-let trace_pcm : FStar.PCM.pcm trace_pcm_t = FP.fp_pcm trace_preorder
-
-//
-// Current state of a trace
-//
-// We use UnInitialized as the current state of empty trace
-//
-noextract
-let current_state (t:trace) : g_session_state =
-  match t with
-  | [] -> G_UnInitialized
-  | hd::_ ->
-    match hd with
-    | [] -> G_UnInitialized
-    | s::_ -> s
-
-//
-// Given a trace t, valid_transition t s means that
-//   current state of t may go to s in the state machine
-//
-noextract
-let valid_transition (t:trace) (s:g_session_state) : prop =
-  next (current_state t) s
-
-//
-// The next trace after a transition
-//
-noextract
-let next_trace (t:trace) (s:g_session_state { valid_transition t s }) : trace =
-  match t with
-  | [] -> [[s]]
-  | hd::tl ->
-    match hd with
-    | [] -> [s]::t
-    | l -> (s::l)::t
-
-//
-// A frame preserving update in the trace PCM,
-//   given a valid transition
-//
-noextract
-let mk_frame_preserving_upd
-  (t:hist trace_preorder)
-  (s:g_session_state { valid_transition t s })
-  : FStar.PCM.frame_preserving_upd trace_pcm (Some 1.0R, t) (Some 1.0R, next_trace t s) =
-  fun _ -> Some 1.0R, next_trace t s
-
-//
-// A snapshot of the trace PCM is the trace with no permission
-//
-noextract
-let snapshot (x:trace_pcm_t) : trace_pcm_t = None, snd x
-
-let snapshot_idempotent (x:trace_pcm_t)
-  : Lemma (snapshot x == snapshot (snapshot x)) = ()
-
-let snapshot_duplicable (x:trace_pcm_t)
-  : Lemma
-      (requires True)
-      (ensures x `FStar.PCM.composable trace_pcm` snapshot x) = ()
-
-let full_perm_empty_history_compatible ()
-  : Lemma (FStar.PCM.compatible trace_pcm (Some 1.0R, []) (Some 1.0R, [])) = ()
-
-noextract
-type pcm_t : Type u#1 = PM.map sid_t trace_pcm_t
-
-//
-// The PCM for the DPE state is a map pcm with sid_t keys
-//   and pointwise trace_pcm
-noextract
-let pcm : PCM.pcm pcm_t = PM.pointwise sid_t trace_pcm
-
-[@@ erasable]
-type gref = ghost_pcm_ref pcm
-
-noextract
-let emp_trace : trace = []
-
-noextract
-let singleton (sid:sid_t) (p:perm) (t:trace) : GTot pcm_t =
-  Map.upd (Map.const (None, emp_trace)) sid (Some p, t)
-
-//
-// The main permission we provide to the client,
-//   to capture the session history for a sid
-//
-noextract
-let sid_pts_to (r:gref) (sid:sid_t) (t:trace) : vprop =
-  ghost_pcm_pts_to r (singleton sid 0.5R t)
-
-noextract
-type pht_t = PHT.pht_t sid_t session_state
-
-//
-// Towards the global state invariant
-//
-
-let session_state_related (s:session_state) (gs:g_session_state) : v:vprop { is_small v } =
-  match s, gs with
-  | SessionStart, G_SessionStart
-  | InUse, G_InUse _
-  | SessionClosed, G_SessionClosed _
-  | SessionError, G_SessionError _ -> emp
-
-  | Available {context}, G_Available repr -> context_perm context repr
-
-  | _ -> pure False
-
-//
-// Invariant for sessions that have been started
-//
-let session_state_perm (r:gref) (pht:pht_t) (sid:sid_t) : v:vprop { is_small v } =
-  exists* (s:session_state) (t:trace).
-    pure (PHT.lookup pht sid == Some s) **
-    sid_pts_to r sid t **
-    session_state_related s (current_state t)
-
-//
-// We have to do this UInt.fits since the OnRange is defined for nat keys,
-//   if we parameterized it over a typeclass, we can directly use u32 keys
-//   and this should go away
-//
-let session_perm (r:gref) (pht:pht_t) (sid:nat) =
-  if UInt.fits sid 32
-  then session_state_perm r pht (U32.uint_to_t sid)
-  else emp
-
-noextract
-let map_literal (f:sid_t -> trace_pcm_t) : pcm_t = Map.map_literal f
-
-noextract
-let all_sids_unused : pcm_t = map_literal (fun _ -> Some 1.0R, emp_trace)
-
-let sids_above_unused (s:sid_t) : GTot pcm_t = map_literal (fun sid ->
-  if U32.lt sid s then None, emp_trace
-  else Some 1.0R, emp_trace)
-
-//
-// Main invariant
-//
-let inv (r:gref) (s:option st) : vprop =
-  match s with
-  //
-  // Global state is not initialized,
-  //   all the sessions are unused
-  //
-  | None -> ghost_pcm_pts_to r all_sids_unused
-  
-  //
-  // Global state has been initialized
-  //
-  | Some s ->
-    //
-    // sids above counter are unused
-    //
-    ghost_pcm_pts_to r (sids_above_unused s.st_ctr) **
-    
-    //
-    // For sids below counter, we have the session state perm
-    //
-    (exists* pht. models s.st_tbl pht **
-                  on_range (session_perm r pht) 0 (U32.v s.st_ctr))
-
-let inv_is_small (r:gref) (s:option st)
-  : Lemma (is_small (inv r s))
-          [SMTPat (is_small (inv r s))] = ()
-
-
-//
-// The DPE API
-//
-
-let open_session_client_perm (r:gref) (s:option sid_t) : vprop =
-  match s with
-  | None -> emp
-  | Some s ->
-    exists* t. sid_pts_to r s t ** pure (current_state t == G_SessionStart)
-
-val open_session (r:gref) (m:mutex (option st))
-  : stt (mutex (option st) & option sid_t)
-        (requires mutex_live m (inv r))
-        (ensures fun b ->
-           mutex_live (fst b) (inv r) **
-           open_session_client_perm r (snd b) **
-           pure (fst b == m))
-
-noextract
-let trace_valid_for_initialize_context (t:trace) : prop =
-  current_state t == G_SessionStart
-
-let initialize_context_client_perm (r:gref) (sid:sid_t) (uds:Seq.seq U8.t) =
-  exists* t. sid_pts_to r sid t **
-             pure (current_state t == G_Available (Engine_context_repr uds))
-
-val initialize_context (r:gref) (m:mutex (option st))
-  (sid:sid_t) 
-  (t:G.erased trace { trace_valid_for_initialize_context t })
-  (#p:perm) (#uds_bytes:Ghost.erased (Seq.seq U8.t))
-  (uds:A.larray U8.t (SZ.v uds_len)) 
-  : stt (mutex (option st) & ctxt_hndl_t)
-        (requires
-           mutex_live m (inv r) **
-           A.pts_to uds #p uds_bytes **
-           sid_pts_to r sid t)
-        (ensures fun b ->
-           mutex_live (fst b) (inv r) **
-           A.pts_to uds #p uds_bytes **
-           initialize_context_client_perm r sid uds_bytes)
-
-noextract
-let trace_and_record_valid_for_derive_child (t:trace) (r:repr_t) : prop =
-  match current_state t, r with
-  | G_Available (Engine_context_repr _), Engine_repr _
-  | G_Available (L0_context_repr _), L0_repr _ -> True
-  | _ -> False
-
-noextract
-let derive_child_post_trace (r:repr_t) (t:trace) =
-  match r, current_state t with
-  | Engine_repr r, G_Available (L0_context_repr lrepr)
-  | L0_repr r, G_Available (L1_context_repr lrepr) -> lrepr.repr == r
-  | _ -> False
-
-let derive_child_client_perm (r:gref) (sid:sid_t) (t0:trace) (repr:repr_t) (c:option ctxt_hndl_t)
-  : vprop =
-  match c with
-  | None ->
-    exists* t1. sid_pts_to r sid t1 **
-                pure (current_state t1 == G_SessionError (G_InUse (current_state t0)))
-  | Some _ ->
-    exists* t1. sid_pts_to r sid t1 **
-                pure (derive_child_post_trace repr t1)
-
-val derive_child (r:gref) (m:mutex (option st)) (sid:sid_t) (ctxt_hndl:ctxt_hndl_t)
-  (t:G.erased trace)
-  (record:record_t)
-  (#rrepr:erased repr_t { trace_and_record_valid_for_derive_child t rrepr })
-  (#p:perm)
-  : stt (mutex (option st) & record_t & option ctxt_hndl_t)
-        (requires
-           mutex_live m (inv r) **
-           record_perm record p rrepr **
-           sid_pts_to r sid t)
-        (ensures fun b ->
-           mutex_live (tfst b) (inv r) **
-           record_perm (tsnd b) p rrepr **
-           derive_child_client_perm r sid t rrepr (tthd b))
-
-
-noextract
-let trace_valid_for_close (t:trace) : prop =
-  match current_state t with
-  | G_UnInitialized
-  | G_SessionClosed _
-  | G_InUse _ -> False
-  | _ -> True
-
-let session_closed_client_perm (r:gref) (sid:sid_t) (t0:trace) =
-  exists* t1. sid_pts_to r sid t1 **
-              pure (current_state t1 == G_SessionClosed (G_InUse (current_state t0)))
-
-val close_session
-  (r:gref)
-  (m:mutex (option st))
-  (sid:sid_t)
-  (t:G.erased trace { trace_valid_for_close t })
-  : stt (mutex (option st))
-        (requires
-           mutex_live m (inv r) **
-           sid_pts_to r sid t)
-        (ensures fun m ->
-           mutex_live m (inv r) **
-           session_closed_client_perm r sid t)
-
 assume val sid_hash : sid_t -> SZ.t
 
 [@@ Rust_const_fn]
@@ -479,13 +55,13 @@ assume val sid_hash : sid_t -> SZ.t
 fn initialize_global_state ()
   requires emp
   returns b:(gref & mutex (option st))
-  ensures mutex_live (snd b) (inv (fst b))
+  ensures mutex_live (snd b) (dpe_inv (fst b))
 {
   let r = ghost_alloc #_ #pcm all_sids_unused;
   with _v. rewrite (ghost_pcm_pts_to r (G.reveal (G.hide _v))) as
                    (ghost_pcm_pts_to r _v);
-  fold (inv r None);
-  let m = new_mutex (inv r) None;
+  fold (dpe_inv r None);
+  let m = new_mutex (dpe_inv r) None;
   let s = ((r, m) <: gref & mutex (option st));
   rewrite each
     r as fst s,
@@ -677,12 +253,12 @@ let emp_to_start_valid () : Lemma (valid_transition emp_trace G_SessionStart) = 
 #push-options "--fuel 0 --ifuel 2 --split_queries no --z3rlimit_factor 2"
 ```pulse
 fn __open_session (r:gref) (s:st)
-  requires inv r (Some s)
+  requires dpe_inv r (Some s)
   returns b:(st & option sid_t)
-  ensures inv r (Some (fst b)) **
+  ensures dpe_inv r (Some (fst b)) **
           open_session_client_perm r (snd b)
 {
-  unfold (inv r (Some s));
+  unfold (dpe_inv r (Some s));
 
   let ctr = s.st_ctr;
   let tbl = s.st_tbl;
@@ -704,7 +280,7 @@ fn __open_session (r:gref) (s:st)
       rewrite each
         ctr as (fst ret).st_ctr,
         tbl as (fst ret).st_tbl;
-      fold (inv r (Some (fst ret)));
+      fold (dpe_inv r (Some (fst ret)));
       rewrite emp as (open_session_client_perm r (snd ret));
       ret
     }
@@ -737,7 +313,7 @@ fn __open_session (r:gref) (s:st)
         rewrite each
           ctr1 as (fst ret).st_ctr,
           tbl1 as (fst ret).st_tbl;
-        fold (inv r (Some (fst ret)));
+        fold (dpe_inv r (Some (fst ret)));
         fold (open_session_client_perm r (Some ctr));
         ret
       } else {
@@ -747,7 +323,7 @@ fn __open_session (r:gref) (s:st)
           tbl1 as (fst ret).st_tbl,
           pht1 as pht,
           ctr as (fst ret).st_ctr;
-        fold (inv r (Some (fst ret)));
+        fold (dpe_inv r (Some (fst ret)));
         rewrite emp as (open_session_client_perm r (snd ret));
         ret
       }
@@ -759,9 +335,9 @@ fn __open_session (r:gref) (s:st)
 
 ```pulse
 fn maybe_mk_session_tbl (r:gref) (sopt:option st)
-  requires inv r sopt
+  requires dpe_inv r sopt
   returns s:st
-  ensures inv r (Some s)
+  ensures dpe_inv r (Some s)
 {
   match sopt {
     None -> {
@@ -773,7 +349,7 @@ fn maybe_mk_session_tbl (r:gref) (sopt:option st)
 
       rewrite each tbl as s.st_tbl;
 
-      unfold inv;
+      unfold dpe_inv;
       assert (pure (Map.equal all_sids_unused (sids_above_unused s.st_ctr)));
       rewrite (ghost_pcm_pts_to r all_sids_unused) as
               (ghost_pcm_pts_to r (sids_above_unused s.st_ctr));
@@ -783,7 +359,7 @@ fn maybe_mk_session_tbl (r:gref) (sopt:option st)
       rewrite (on_range (session_perm r pht) 0 0) as
               (on_range (session_perm r pht) 0 (U32.v s.st_ctr));
   
-      fold (inv r (Some s));
+      fold (dpe_inv r (Some s));
       s
     }
     Some s -> {
@@ -795,9 +371,9 @@ fn maybe_mk_session_tbl (r:gref) (sopt:option st)
 
 ```pulse
 fn open_session (r:gref) (m:mutex (option st))
-  requires mutex_live m (inv r)
+  requires mutex_live m (dpe_inv r)
   returns b:(mutex (option st) & option sid_t)
-  ensures mutex_live (fst b) (inv r) **
+  ensures mutex_live (fst b) (dpe_inv r) **
           open_session_client_perm r (snd b) **
           pure (fst b == m)
 {
@@ -895,13 +471,13 @@ fn replace_session
   (sst:session_state)
   (gsst:g_session_state { valid_transition t gsst})
 
-  requires mutex_live m (inv r) **
+  requires mutex_live m (dpe_inv r) **
            sid_pts_to r sid t **
            session_state_related sst gsst
 
   returns b:(mutex (option st) & session_state)
 
-  ensures mutex_live (fst b) (inv r) **
+  ensures mutex_live (fst b) (dpe_inv r) **
           session_state_related (snd b) (current_state t) **
           sid_pts_to r sid (next_trace t gsst)
 {
@@ -909,13 +485,13 @@ fn replace_session
   let sopt = M.replace mg None;
   match sopt {
     None -> {
-      unfold (inv r None);
+      unfold (dpe_inv r None);
       unfold sid_pts_to;
       gather_ r all_sids_unused (singleton sid 0.5R t);
       unreachable ()
     }
     Some s -> {
-      unfold (inv r (Some s));
+      unfold (dpe_inv r (Some s));
       let ctr = s.st_ctr;
       let tbl = s.st_tbl;
       rewrite each
@@ -965,7 +541,7 @@ fn replace_session
               rewrite each
                 ctr as s.st_ctr,
                 tbl as s.st_tbl;
-              fold (inv r (Some s));
+              fold (dpe_inv r (Some s));
               mg := Some s;
               unlock m mg;
               let ret = (m, st);
@@ -1064,13 +640,13 @@ fn initialize_context (r:gref) (m:mutex (option st))
   (#p:perm) (#uds_bytes:Ghost.erased (Seq.seq U8.t))
   (uds:A.larray U8.t (SZ.v uds_len)) 
                        
-  requires mutex_live m (inv r) **
+  requires mutex_live m (dpe_inv r) **
            A.pts_to uds #p uds_bytes **
            sid_pts_to r sid t
 
   returns b:(mutex (option st) & ctxt_hndl_t)
 
-  ensures mutex_live (fst b) (inv r) **
+  ensures mutex_live (fst b) (dpe_inv r) **
           A.pts_to uds #p uds_bytes **
           initialize_context_client_perm r sid uds_bytes
 {
@@ -1539,11 +1115,11 @@ fn derive_child (r:gref) (m:mutex (option st)) (sid:sid_t) (ctxt_hndl:ctxt_hndl_
   (record:record_t)
   (#rrepr:erased repr_t { trace_and_record_valid_for_derive_child t rrepr })
   (#p:perm)
-  requires mutex_live m (inv r) **
+  requires mutex_live m (dpe_inv r) **
            record_perm record p rrepr **
            sid_pts_to r sid t
   returns b:(mutex (option st) & record_t & option ctxt_hndl_t)
-  ensures mutex_live (tfst b) (inv r) **
+  ensures mutex_live (tfst b) (dpe_inv r) **
           record_perm (tsnd b) p rrepr **
           derive_child_client_perm r sid t rrepr (tthd b)
 {
@@ -1674,10 +1250,10 @@ fn destroy_session_state (s:session_state) (t:G.erased trace)
 ```pulse
 fn close_session (r:gref) (m:mutex (option st)) (sid:sid_t)
   (t:G.erased trace { trace_valid_for_close t })
-  requires mutex_live m (inv r) **
+  requires mutex_live m (dpe_inv r) **
            sid_pts_to r sid t
   returns m:mutex (option st)
-  ensures mutex_live m (inv r) **
+  ensures mutex_live m (dpe_inv r) **
           session_closed_client_perm r sid t
 {
   rewrite emp as (session_state_related InUse (G_InUse (current_state t)));
