pulse/share/pulse/examples/dice/dpe/DPE.fsti
@@ -1,0 +1,467 @@
+(*
+   Copyright 2023 Microsoft Research
+
+   Licensed under the Apache License, Version 2.0 (the "License");
+   you may not use this file except in compliance with the License.
+   You may obtain a copy of the License at
+
+       http://www.apache.org/licenses/LICENSE-2.0
+
+   Unless required by applicable law or agreed to in writing, software
+   distributed under the License is distributed on an "AS IS" BASIS,
+   WITHOUT WARRANTIES OR CONDITIONS OF ANY KIND, either express or implied.
+   See the License for the specific language governing permissions and
+   limitations under the License.
+*)
+
+module DPE
+open Pulse.Lib.Pervasives
+open DPETypes
+open HACL
+open X509
+open EngineTypes
+open EngineCore
+open L0Types
+open L0Core
+
+module G = FStar.Ghost
+module PCM = FStar.PCM
+module SZ = FStar.SizeT
+module U8 = FStar.UInt8
+module U32 = FStar.UInt32
+module PM = Pulse.Lib.PCMMap
+module FP = Pulse.Lib.PCM.FractionalPreorder
+module M = Pulse.Lib.Mutex
+module A = Pulse.Lib.Array
+module HT = Pulse.Lib.HashTable
+module PHT = Pulse.Lib.HashTable.Spec
+
+open PulseCore.Preorder
+open Pulse.Lib.OnRange
+open Pulse.Lib.HashTable.Type
+open Pulse.Lib.HashTable
+open Pulse.Lib.Mutex
+
+//
+// Concrete state setup
+//
+
+type ctxt_hndl_t = U32.t
+
+type sid_t : eqtype = U32.t
+
+//
+// A session may be in one of the following states
+//
+// InUse is never returned to the client
+//
+[@@ Rust_derive "Clone"]
+noeq
+type session_state =
+  | SessionStart
+  | Available { handle:ctxt_hndl_t; context:context_t }
+  | InUse
+  | SessionClosed
+  | SessionError
+
+type ht_t = ht_t sid_t session_state
+
+//
+// DPE state
+// A counter for next sid
+//   and a hashtable mapping sids to session state
+//
+noeq
+type st = { st_ctr:sid_t; st_tbl:ht_t; }
+
+
+//
+// Ghost state set up
+//
+
+//
+// Ghost session state
+//
+// Has a 1-1 correspondence with the concrete session state
+//   except it has an G_UnInitialized
+//
+[@@ erasable]
+noeq
+type g_session_state : Type u#1 =
+  | G_UnInitialized : g_session_state
+  | G_SessionStart : g_session_state
+  | G_Available : repr:context_repr_t -> g_session_state
+  | G_InUse : g_session_state -> g_session_state
+  | G_SessionClosed : g_session_state -> g_session_state
+  | G_SessionError : g_session_state -> g_session_state
+
+//
+// A relation between context reprs that follow each other
+//
+// L0 repr should use the same UDS as the engine repr,
+//   and L1 repr should use the same CDI as the L0 repr
+//
+noextract
+let next_repr (r1 r2:context_repr_t) : prop =
+  match r1, r2 with
+  | Engine_context_repr uds, L0_context_repr l0_repr ->
+    uds == l0_repr.uds
+  | L0_context_repr l0_repr, L1_context_repr l1_repr ->
+    l0_repr.cdi == l1_repr.cdi
+  | _ -> False
+
+//
+// State machine
+//
+noextract
+let rec next (s0 s1:g_session_state) : prop =
+  match s0, s1 with
+  //
+  // UnInitialized may only go to SessionStart
+  // No other incoming/outgoing edges to/from it
+  //
+  | G_UnInitialized, G_SessionStart -> True
+  | G_UnInitialized, _
+  | _, G_UnInitialized -> False
+
+  //
+  // SessionStart may go to Available with engine repr
+  //
+  | G_SessionStart, G_Available (Engine_context_repr _) -> True
+
+  //
+  // Available r0 may go to Available r1,
+  //   as long as repr r1 follows repr r0
+  //
+  | G_Available r0, G_Available r1 -> next_repr r0 r1
+
+  //
+  // SessionClosed is a terminal state
+  //
+  | G_SessionClosed _, _ -> False
+
+  //
+  // From any state we can go to InUse, SessionClosed, or SessionError
+  //
+  // These states capture the previous state
+  //
+  | _, G_InUse s -> s == s0
+  | _, G_SessionClosed s
+  | _, G_SessionError s -> s == s0
+
+  //
+  // From InUse s we can go to s1, as long as s can go to s1
+  //
+  | G_InUse s, s1 -> next s s1
+
+  | _ -> False
+
+
+//
+// Defining traces
+//
+
+noextract
+let rec well_formed_trace (l:list g_session_state) : prop =
+  match l with
+  | []
+  | [G_SessionStart] -> True
+  | s1::s0::tl -> next s0 s1 /\ well_formed_trace (s0::tl)
+  | _ -> False
+
+noextract
+type trace_elt : Type u#1 = l:list g_session_state { well_formed_trace l }
+
+noextract
+let trace_extension (t0 t1:trace_elt) : prop =
+  Cons? t1 /\ t0 == List.Tot.tail t1
+
+noextract
+let trace_preorder : FStar.Preorder.preorder trace_elt =
+  FStar.ReflexiveTransitiveClosure.closure trace_extension
+
+noextract
+type trace = hist trace_preorder
+
+noextract
+type trace_pcm_t : Type u#1 = FP.pcm_carrier trace_preorder
+
+//
+// Trace PCM is fractional preorder PCM,
+//   with trace preorder
+//
+noextract
+let trace_pcm : FStar.PCM.pcm trace_pcm_t = FP.fp_pcm trace_preorder
+
+//
+// Current state of a trace
+//
+// We use UnInitialized as the current state of empty trace
+//
+noextract
+let current_state (t:trace) : g_session_state =
+  match t with
+  | [] -> G_UnInitialized
+  | hd::_ ->
+    match hd with
+    | [] -> G_UnInitialized
+    | s::_ -> s
+
+//
+// Given a trace t, valid_transition t s means that
+//   current state of t may go to s in the state machine
+//
+noextract
+let valid_transition (t:trace) (s:g_session_state) : prop =
+  next (current_state t) s
+
+//
+// The next trace after a transition
+//
+noextract
+let next_trace (t:trace) (s:g_session_state { valid_transition t s }) : trace =
+  match t with
+  | [] -> [[s]]
+  | hd::tl ->
+    match hd with
+    | [] -> [s]::t
+    | l -> (s::l)::t
+
+//
+// A frame preserving update in the trace PCM,
+//   given a valid transition
+//
+noextract
+let mk_frame_preserving_upd
+  (t:hist trace_preorder)
+  (s:g_session_state { valid_transition t s })
+  : FStar.PCM.frame_preserving_upd trace_pcm (Some 1.0R, t) (Some 1.0R, next_trace t s) =
+  fun _ -> Some 1.0R, next_trace t s
+
+//
+// A snapshot of the trace PCM is the trace with no permission
+//
+noextract
+let snapshot (x:trace_pcm_t) : trace_pcm_t = None, snd x
+
+let snapshot_idempotent (x:trace_pcm_t)
+  : Lemma (snapshot x == snapshot (snapshot x)) = ()
+
+let snapshot_duplicable (x:trace_pcm_t)
+  : Lemma
+      (requires True)
+      (ensures x `FStar.PCM.composable trace_pcm` snapshot x) = ()
+
+let full_perm_empty_history_compatible ()
+  : Lemma (FStar.PCM.compatible trace_pcm (Some 1.0R, []) (Some 1.0R, [])) = ()
+
+noextract
+type pcm_t : Type u#1 = PM.map sid_t trace_pcm_t
+
+//
+// The PCM for the DPE state is a map pcm with sid_t keys
+//   and pointwise trace_pcm
+noextract
+let pcm : PCM.pcm pcm_t = PM.pointwise sid_t trace_pcm
+
+[@@ erasable]
+type gref = ghost_pcm_ref pcm
+
+noextract
+let emp_trace : trace = []
+
+noextract
+let singleton (sid:sid_t) (p:perm) (t:trace) : GTot pcm_t =
+  Map.upd (Map.const (None, emp_trace)) sid (Some p, t)
+
+//
+// The main permission we provide to the client,
+//   to capture the session history for a sid
+//
+noextract
+let sid_pts_to (r:gref) (sid:sid_t) (t:trace) : vprop =
+  ghost_pcm_pts_to r (singleton sid 0.5R t)
+
+noextract
+type pht_t = PHT.pht_t sid_t session_state
+
+//
+// Towards the global state invariant
+//
+
+let session_state_related (s:session_state) (gs:g_session_state) : v:vprop { is_small v } =
+  match s, gs with
+  | SessionStart, G_SessionStart
+  | InUse, G_InUse _
+  | SessionClosed, G_SessionClosed _
+  | SessionError, G_SessionError _ -> emp
+
+  | Available {context}, G_Available repr -> context_perm context repr
+
+  | _ -> pure False
+
+//
+// Invariant for sessions that have been started
+//
+let session_state_perm (r:gref) (pht:pht_t) (sid:sid_t) : v:vprop { is_small v } =
+  exists* (s:session_state) (t:trace).
+    pure (PHT.lookup pht sid == Some s) **
+    sid_pts_to r sid t **
+    session_state_related s (current_state t)
+
+//
+// We have to do this UInt.fits since the OnRange is defined for nat keys,
+//   if we parameterized it over a typeclass, we can directly use u32 keys
+//   and this should go away
+//
+let session_perm (r:gref) (pht:pht_t) (sid:nat) =
+  if UInt.fits sid 32
+  then session_state_perm r pht (U32.uint_to_t sid)
+  else emp
+
+noextract
+let map_literal (f:sid_t -> trace_pcm_t) : pcm_t = Map.map_literal f
+
+noextract
+let all_sids_unused : pcm_t = map_literal (fun _ -> Some 1.0R, emp_trace)
+
+let sids_above_unused (s:sid_t) : GTot pcm_t = map_literal (fun sid ->
+  if U32.lt sid s then None, emp_trace
+  else Some 1.0R, emp_trace)
+
+//
+// Main invariant
+//
+let dpe_inv (r:gref) (s:option st) : vprop =
+  match s with
+  //
+  // Global state is not initialized,
+  //   all the sessions are unused
+  //
+  | None -> ghost_pcm_pts_to r all_sids_unused
+  
+  //
+  // Global state has been initialized
+  //
+  | Some s ->
+    //
+    // sids above counter are unused
+    //
+    ghost_pcm_pts_to r (sids_above_unused s.st_ctr) **
+    
+    //
+    // For sids below counter, we have the session state perm
+    //
+    (exists* pht. models s.st_tbl pht **
+                  on_range (session_perm r pht) 0 (U32.v s.st_ctr))
+
+let inv_is_small (r:gref) (s:option st)
+  : Lemma (is_small (dpe_inv r s))
+          [SMTPat (is_small (dpe_inv r s))] = ()
+
+
+//
+// The DPE API
+//
+
+let open_session_client_perm (r:gref) (s:option sid_t) : vprop =
+  match s with
+  | None -> emp
+  | Some s ->
+    exists* t. sid_pts_to r s t ** pure (current_state t == G_SessionStart)
+
+val open_session (r:gref) (m:mutex (option st))
+  : stt (mutex (option st) & option sid_t)
+        (requires mutex_live m (dpe_inv r))
+        (ensures fun b ->
+           mutex_live (fst b) (dpe_inv r) **
+           open_session_client_perm r (snd b) **
+           pure (fst b == m))
+
+noextract
+let trace_valid_for_initialize_context (t:trace) : prop =
+  current_state t == G_SessionStart
+
+let initialize_context_client_perm (r:gref) (sid:sid_t) (uds:Seq.seq U8.t) =
+  exists* t. sid_pts_to r sid t **
+             pure (current_state t == G_Available (Engine_context_repr uds))
+
+val initialize_context (r:gref) (m:mutex (option st))
+  (sid:sid_t) 
+  (t:G.erased trace { trace_valid_for_initialize_context t })
+  (#p:perm) (#uds_bytes:Ghost.erased (Seq.seq U8.t))
+  (uds:A.larray U8.t (SZ.v uds_len)) 
+  : stt (mutex (option st) & ctxt_hndl_t)
+        (requires
+           mutex_live m (dpe_inv r) **
+           A.pts_to uds #p uds_bytes **
+           sid_pts_to r sid t)
+        (ensures fun b ->
+           mutex_live (fst b) (dpe_inv r) **
+           A.pts_to uds #p uds_bytes **
+           initialize_context_client_perm r sid uds_bytes)
+
+noextract
+let trace_and_record_valid_for_derive_child (t:trace) (r:repr_t) : prop =
+  match current_state t, r with
+  | G_Available (Engine_context_repr _), Engine_repr _
+  | G_Available (L0_context_repr _), L0_repr _ -> True
+  | _ -> False
+
+noextract
+let derive_child_post_trace (r:repr_t) (t:trace) =
+  match r, current_state t with
+  | Engine_repr r, G_Available (L0_context_repr lrepr)
+  | L0_repr r, G_Available (L1_context_repr lrepr) -> lrepr.repr == r
+  | _ -> False
+
+let derive_child_client_perm (r:gref) (sid:sid_t) (t0:trace) (repr:repr_t) (c:option ctxt_hndl_t)
+  : vprop =
+  match c with
+  | None ->
+    exists* t1. sid_pts_to r sid t1 **
+                pure (current_state t1 == G_SessionError (G_InUse (current_state t0)))
+  | Some _ ->
+    exists* t1. sid_pts_to r sid t1 **
+                pure (derive_child_post_trace repr t1)
+
+val derive_child (r:gref) (m:mutex (option st)) (sid:sid_t) (ctxt_hndl:ctxt_hndl_t)
+  (t:G.erased trace)
+  (record:record_t)
+  (#rrepr:erased repr_t { trace_and_record_valid_for_derive_child t rrepr })
+  (#p:perm)
+  : stt (mutex (option st) & record_t & option ctxt_hndl_t)
+        (requires
+           mutex_live m (dpe_inv r) **
+           record_perm record p rrepr **
+           sid_pts_to r sid t)
+        (ensures fun b ->
+           mutex_live (tfst b) (dpe_inv r) **
+           record_perm (tsnd b) p rrepr **
+           derive_child_client_perm r sid t rrepr (tthd b))
+
+
+noextract
+let trace_valid_for_close (t:trace) : prop =
+  match current_state t with
+  | G_UnInitialized
+  | G_SessionClosed _
+  | G_InUse _ -> False
+  | _ -> True
+
+let session_closed_client_perm (r:gref) (sid:sid_t) (t0:trace) =
+  exists* t1. sid_pts_to r sid t1 **
+              pure (current_state t1 == G_SessionClosed (G_InUse (current_state t0)))
+
+val close_session
+  (r:gref)
+  (m:mutex (option st))
+  (sid:sid_t)
+  (t:G.erased trace { trace_valid_for_close t })
+  : stt (mutex (option st))
+        (requires
+           mutex_live m (dpe_inv r) **
+           sid_pts_to r sid t)
+        (ensures fun m ->
+           mutex_live m (dpe_inv r) **
+           session_closed_client_perm r sid t)
